ast to cfg transformation (WIP)

Cfg.dfy
@@ -61,9 +61,209 @@ module BoogieCfg {
     var successors := g.successors[n];
 
     if |successors| == 0 then 
-      WpShallowSimpleCmdConj(a, g.blocks[n], post)
+      WpShallowSimpleCmdSeq(a, g.blocks[n], post)
     else 
-      WpShallowSimpleCmdConj(a, g.blocks[n], WpCfgConjunction(a, g, successors, post, cover - {n}))
+      WpShallowSimpleCmdSeq(a, g.blocks[n], WpCfgConjunction(a, g, successors, post, cover - {n}))
   }
+
+  /***********************************************************************************
+                    Alternatives (more liberal conditions on graphs)
+  ************************************************************************************
+  ************************************************************************************
+  ************************************************************************************/
+
+  function CfgWfAlt(g: Cfg, notRecorded: set<BlockId>) : bool
+  {
+    g.blocks.Keys == g.successors.Keys &&
+    g.entry in g.blocks.Keys &&
+    (forall blockId :: blockId in g.blocks.Keys ==> 
+      (forall i :: 0 <= i < |g.successors[blockId]| ==> g.successors[blockId][i] in g.blocks.Keys + notRecorded))
+  }
+
+  type SuccessorRel = map<BlockId, seq<BlockId>>
+
+  function IsAcyclicSeqAlt(r: SuccessorRel, ns: seq<BlockId>, cover: set<BlockId>) : bool
+    decreases cover, 1, ns
+  {
+    |ns| != 0 ==> ( IsAcyclicAlt(r, ns[0], cover) && IsAcyclicSeqAlt(r, ns[1..], cover) )
+  }
+
+  function IsAcyclicAlt(r: SuccessorRel, n: BlockId, cover: set<BlockId>) : bool
+    decreases cover, 0
+  {
+    n in r.Keys ==> ( n in cover && IsAcyclicSeqAlt(r, r[n], cover - {n}) )
+  }
+
+  datatype WpPostCfg<!A> = WpPostCfg(normal: Predicate<A>, exceptional: map<BlockId, Predicate<A>>)
+
+  function WpCfgConjunctionAlt<A(!new)>(
+    a: absval_interp<A>, 
+    g: Cfg, 
+    ns: seq<BlockId>, 
+    post: Predicate<A>, 
+    cover: set<BlockId>) : Predicate<A>
+    requires g.blocks.Keys == g.successors.Keys
+    requires IsAcyclicSeqAlt(g.successors, ns, cover)
+    decreases cover, 1, ns
+  { s =>
+      if |ns| == 0 then Some(true)
+      else 
+        var res1 :- WpCfgAlt(a, g, ns[0], post, cover)(s);
+        var res2 :- WpCfgConjunctionAlt(a, g, ns[1..], post, cover)(s);
+        Some(res1 && res2)
+  }
+
+  function WpCfgAlt<A(!new)>(a: absval_interp<A>, g: Cfg, n: BlockId, post: Predicate<A>, cover: set<BlockId>) : Predicate<A>
+    requires g.blocks.Keys == g.successors.Keys
+    requires IsAcyclicAlt(g.successors, n, cover)
+    decreases cover, 0
+  {
+    if !(n in g.blocks.Keys) then
+      post
+    else 
+      var successors := g.successors[n];
+      if |successors| == 0 then 
+        WpShallowSimpleCmdSeq(a, g.blocks[n], post)
+      else 
+        WpShallowSimpleCmdSeq(a, g.blocks[n], WpCfgConjunctionAlt(a, g, successors, post, cover - {n}))
+  }
+
+  /** Lemmas */
+  lemma IsAcyclicSeqLargerCover(r: SuccessorRel, ns: seq<BlockId>, cover1: set<BlockId>, cover2: set<BlockId>)
+    requires cover1 <= cover2 && IsAcyclicSeqAlt(r, ns, cover1)
+    ensures IsAcyclicSeqAlt(r, ns, cover2)
+    decreases cover1, 1, ns
+  {
+    if |ns| != 0 {
+      IsAcyclicLargerCover(r, ns[0], cover1, cover2); 
+      IsAcyclicSeqLargerCover(r, ns[1..], cover1, cover2);
+    }
+  }
+
+  lemma IsAcyclicLargerCover(r: SuccessorRel, n: BlockId, cover1: set<BlockId>, cover2: set<BlockId>)
+    requires cover1 <= cover2 && IsAcyclicAlt(r, n, cover1)
+    ensures IsAcyclicAlt(r, n, cover2)
+    decreases cover1, 0
+  {
+    if n in r.Keys {
+      IsAcyclicSeqLargerCover(r, r[n], cover1 - {n}, cover2 - {n});
+    }
+  }
+
+  lemma IsAcyclicSeqMerge(
+    r1: SuccessorRel, 
+    r2: SuccessorRel, 
+    ns1: seq<BlockId>,
+    n2Entry: BlockId,
+    cover1: set<BlockId>, 
+    cover2: set<BlockId>)
+    requires cover1 !! cover2
+    requires r1.Keys !! r2.Keys
+    requires IsAcyclicSeqAlt(r1, ns1, cover1)
+    requires IsAcyclicAlt(r2, n2Entry, cover2)
+
+    requires 
+      (forall i :: 0 <= i < |ns1| ==> 
+             ns1[i] in r1.Keys || ns1[i] == n2Entry)
+
+    requires !(n2Entry in r1.Keys)
+
+    requires 
+      (forall i :: 0 <= i < |ns1| ==> 
+             ns1[i] in r1.Keys || ns1[i] == n2Entry)
+    // successors in r1 are either n2Entry or blocks recorded in r1
+    requires 
+      forall n1 :: n1 in r1.Keys ==>   
+        (forall i :: 0 <= i < |r1[n1]| ==> (r1[n1][i] == n2Entry || r1[n1][i] in r1.Keys))
+
+    // successors in r2 are not recorded in r1
+    requires
+      forall n2 :: n2 in r2.Keys ==>   
+        (forall i :: 0 <= i < |r2[n2]| ==> !(r2[n2][i] in r1.Keys))
+    ensures IsAcyclicSeqAlt(r1 + r2, ns1, cover1 + cover2)
+    decreases cover1, 1, ns1
+  {
+    if |ns1| != 0 {
+      IsAcyclicMerge(r1, r2, ns1[0], n2Entry, cover1, cover2);
+      IsAcyclicSeqMerge(r1, r2, ns1[1..], n2Entry, cover1, cover2);
+    }
+  }
+
+  lemma IsAcyclicMerge(
+    r1: SuccessorRel, 
+    r2: SuccessorRel, 
+    n1Entry: BlockId,
+    n2Entry: BlockId,
+    cover1: set<BlockId>, 
+    cover2: set<BlockId>)
+    requires cover1 !! cover2
+    requires r1.Keys !! r2.Keys
+    requires IsAcyclicAlt(r1, n1Entry, cover1)
+    requires IsAcyclicAlt(r2, n2Entry, cover2)
+
+    requires n1Entry in r1.Keys || n1Entry == n2Entry
+    requires !(n2Entry in r1.Keys)
+
+    // successors in r1 are either n2Entry or blocks recorded in r1
+    requires 
+      forall n1 :: n1 in r1.Keys ==>   
+        (forall i :: 0 <= i < |r1[n1]| ==> (r1[n1][i] == n2Entry || r1[n1][i] in r1.Keys))
+
+    // successors in r2 are not recorded in r1
+    requires
+      forall n2 :: n2 in r2.Keys ==>   
+        (forall i :: 0 <= i < |r2[n2]| ==> !(r2[n2][i] in r1.Keys))
+    ensures IsAcyclicAlt(r1 + r2, n1Entry, cover1 + cover2)
+    decreases cover1, 0
+  {
+    if n1Entry in r1.Keys {
+      IsAcyclicSeqMerge(r1, r2, r1[n1Entry], n2Entry, cover1 - {n1Entry}, cover2);
+      calc {
+        IsAcyclicSeqAlt(r1 + r2, r1[n1Entry], (cover1 - {n1Entry}) + cover2); 
+      == { assert (cover1 - {n1Entry}) + cover2 == (cover1 + cover2) - {n1Entry}; }
+        IsAcyclicSeqAlt(r1 + r2, r1[n1Entry], (cover1 + cover2) - {n1Entry});
+      }
+    } else {
+      IsAcyclicExtend(r1, r2, n2Entry, cover2);
+      IsAcyclicLargerCover(r1+r2, n2Entry, cover2, cover1 + cover2);
+    }
+  }
+
+  lemma IsAcyclicExtendSeq(r1: SuccessorRel, r2: SuccessorRel, ns: seq<BlockId>, cover: set<BlockId>)
+    requires IsAcyclicSeqAlt(r2, ns, cover)
+    requires (forall i :: 0 <= i < |ns| ==> !(ns[i] in r1.Keys))
+    requires 
+      forall n2 :: n2 in r2.Keys ==>   
+        (forall i :: 0 <= i < |r2[n2]| ==> !(r2[n2][i] in r1.Keys))
+    ensures IsAcyclicSeqAlt(r1+r2, ns, cover)
+    decreases cover, 1, ns
+  {
+    if |ns| != 0 {
+      IsAcyclicExtend(r1, r2, ns[0], cover);
+      IsAcyclicExtendSeq(r1, r2, ns[1..], cover);
+    }
+  }
+  
+  lemma IsAcyclicExtend(r1: SuccessorRel, r2: SuccessorRel, n2Entry: BlockId, cover: set<BlockId>)
+    requires IsAcyclicAlt(r2, n2Entry, cover)
+    requires !(n2Entry in r1.Keys)
+    requires 
+      forall n2 :: n2 in r2.Keys ==>   
+        (forall i :: 0 <= i < |r2[n2]| ==> !(r2[n2][i] in r1.Keys))
+    ensures IsAcyclicAlt(r1+r2, n2Entry, cover)
+    decreases cover, 0
+  {
+    var r := r1 + r2;
+    if(n2Entry in r.Keys) {
+      assert n2Entry in r2.Keys;
+      assert IsAcyclicSeqAlt(r2, r2[n2Entry], cover - {n2Entry});
+
+      IsAcyclicExtendSeq(r1, r2, r2[n2Entry], cover - {n2Entry});
+    }
+  }
+
+  lemma IsAcyclicNodesSubset(r: SuccessorRel, cover: set<BlockId>)
+    requires IsAcyclicAlt(r, cover)
+    ensures r.successor.Keys <= cover
 
 }
